Ported PCUIC to primitive integers in master

pcuic/theories/PCUICAst.v
@@ -1,5 +1,5 @@
 (* Distributed under the terms of the MIT license.   *)
-
+From Coq Require Int63.
 Require Import Coq.Strings.String.
 Require Import Coq.PArith.BinPos.
 Require Import List. Import ListNotations.
@@ -29,7 +29,11 @@ Inductive term : Set :=
                -> term (* discriminee *) -> list (nat * term) (* branches *) -> term
 | tProj      : projection -> term -> term
 | tFix       : mfixpoint term -> nat -> term
-| tCoFix     : mfixpoint term -> nat -> term.
+| tCoFix     : mfixpoint term -> nat -> term
+| tInt       : Int63.int -> term.
+
+(** Primitive integers type, as defined in the standard library. *)
+Definition tInt_type := tConst "Coq.Numbers.Cyclic.Int63.Int63.int"%string [].
 
 Fixpoint mkApps t us :=
   match us with
