pcuic/theories/PCUICInduction.v
@@ -37,6 +37,8 @@ Lemma term_forall_list_ind :
     (forall (s : projection) (t : term), P t -> P (tProj s t)) ->
     (forall (m : mfixpoint term) (n : nat), tFixProp P P m -> P (tFix m n)) ->
     (forall (m : mfixpoint term) (n : nat), tFixProp P P m -> P (tCoFix m n)) ->
+    (forall (i : Int63.int), P (tInt i)) ->
+
     forall t : term, P t.
 Proof.
   intros until t. revert t.
