pcuic/theories/PCUICWcbvEval.v
@@ -95,6 +95,7 @@ Section Wcbv.
       eval f (tConstruct i k u) ->
       Forall2 eval a a' ->
       eval (mkApps f a) (mkApps (tConstruct i k u) a').
+  (* TODO Int values *)
 
   (* | evar ev l l' : evals l l' -> eval (tEvar ev l) (tEvar ev l') *)
   (* | eval_evar ev l : eval (tEvar ev l) (tEvar ev l) (* Lets say it is a value for now *) *)
@@ -171,8 +172,7 @@ Section Wcbv.
 
       forall t t0 : term, eval t t0 -> P t t0.
   Proof.
-    intros P Hbox Hbeta Hlet Hreldef Hrelvar Hcase Hfix Hconst Hproj Hlam Hprod Hind Hindapp Hcstr Hcstrapp Hevar.
-    (* intros P Hbeta Hlet Hreldef Hrelvar Hcase Hfix Hconst Hproj Hlam Hprod Hind Hindapp Hcstr Hcstrapp (* Hcast *). *)
+    intros P Hbeta Hlet Hreldef Hrelvar Hcase Hfix Hconst Hproj Hlam Hprod Hind Hindapp Hcstr Hcstrapp (* Hcast *).
     fix eval_evals_ind 3. destruct 1;
              try match goal with [ H : _ |- _ ] =>
                              match type of H with
